Flapjack.lean
@@ -2,6 +2,7 @@ import Flapjack.Language
 import Flapjack.PanSimp
 import Flapjack.PanStructs
 import Flapjack.PanGlobals
+import Flapjack.Pipeline
 import Flapjack.Tests
 import Flapjack.Static
 import Flapjack.Crepe
